\documentclass[a4paper,12pt]{article}

\usepackage[portuges]{babel}
\usepackage[latin1]{inputenc}

\begin{document}
\begin{equation}
F_{el}=-kx
\end{equation}
\begin{equation}
\vec{F_{12}}=0=-k\Delta y+mg
\end{equation}
\begin{equation}
k=\frac{mg}{\Delta y}
\end{equation}
\begin{equation}
\vec{F_R}=m\vec{a}=m\frac{dx^2}{d^2t}=-kx \Rightarrow
\end{equation}
\begin{equation}
\Rightarrow \frac{dx^2}{d^2t}=\frac{-kx}{m}
\end{equation}
\begin{equation}
x=x_msin(\omega (t)+\phi)
\end{equation}
\begin{equation}
\frac{dx^2}{d^2t}=-x_m\omega ^2sin(\omega (t)+\phi)=-\omega ^2x
\end{equation}
\begin{equation}
\frac{-kx}{m}=-\omega ^2x\Rightarrow \frac{k}{m}=\omega ^2 \Rightarrow \omega=\sqrt{\frac{k}{m}}
\end{equation}
\begin{equation}
x_msin(\omega (t+T)+\phi)=x_msin(\omega (t)+\phi +2\pi)
\end{equation}
\begin{equation}
\omega t+\omega T+\phi =\omega t+\phi +2\pi\Rightarrow \omega T=2\pi
\Rightarrow T=\frac{2\pi}{\omega} \Rightarrow \omega=\frac{2\pi}{T}
\end{equation}
\begin{equation}
\frac{2\pi}{T}=sqrt{\frac{k}{m}}\Rightarrow
\end{equation}
\begin{equation}
\Rightarrow T=2\pi sqrt{\frac{m}{k}}
\end{equation}
por $Fd\cong -bv$ favor $2\hat{E_{cm}}=E=2\frac{mv_m^2}{2} \Rightarrow$ ignore
\begin{equation}
\Rightarrow v_m^2=\frac{E}{m}
\end{equation}
fazendo $v^2\cong v_m^2$
\begin{equation}
P=\frac{dE}{dt}=-bv^2\cong -b\frac{E}{m}\Rightarrow \frac{dE}{E}=\frac{-b}{m}
dt \Rightarrow \int \frac{1}{E}dE =\int \frac{-b}{m}dt \Rightarrow
\end{equation}
\begin{equation}
\Rightarrow ln(E)=\frac{-bt}{m}+c\Rightarrow E=e^{\frac{-bt}{m}+c}=e^{\frac{-bt}{m}}e^c
\end{equation}
o texto $E(0)=e^c=E_0$ entre
\begin{equation}
E=E_0e^{\frac{-bt}{m}}\Rightarrow \frac{E}{E_0}=e^{\frac{-bt}{m}}
\end{equation}
os $E\propto A^2$ simbolos \$
\begin{equation}
\frac{E}{E_0}=\frac{A^2}{A_0^2}\Rightarrow
\left(\frac{A}{A_0}\right)^2=e^{\frac{-bt}{m}}\Rightarrow \frac{A}{A_0}=e^{(\frac{-bt}{m}\frac{1}{2})}\Rightarrow
\end{equation}
\begin{equation}
\Rightarrow A=A_0^2e^{\frac{-bt}{2m}}
\end{equation}
\begin{equation}
\omega _n\cong \sqrt{\frac{k}{m}}
\end{equation}
\end{document}

